theories/Translations/LustreAstToLustre.v
@@ -87,12 +87,13 @@ Record common_temp : Type := {
   Henv: forall x t, Dict.maps_to x t env <-> In (x, t) (n_in ++ n_out ++ n_locals);
 }.
 
-Definition translate_unop (op: Source.unop): { tin & { tout & Target.unop tin tout } } := match op with
+Definition translate_unop {ty} (op: Source.unop): { tin & { tout & Target.unop tin tout } } := match op with
   | Source.Uop_neg => existT _ _ (existT _ _ Target.Uop_neg)
   | Source.Uop_not => existT _ _ (existT _ _ Target.Uop_not)
-  | Source.Uop_pre => existT _ _ (existT _ _ Target.Uop_pre)
+  | Source.Uop_pre => existT _ _ (existT _ _ (@Target.Uop_pre ty))
 end.
-Definition translate_binop (op: Source.binop): { tin1 & { tin2 & { tout & Target.binop tin1 tin2 tout } } } := match op with
+
+Definition translate_binop {ty} (op: Source.binop): { tin1 & { tin2 & { tout & Target.binop tin1 tin2 tout } } } := match op with
   | Source.Bop_and => existT _ _ (existT _ _ (existT _ _ Target.Bop_and))
   | Source.Bop_or => existT _ _ (existT _ _ (existT _ _ Target.Bop_or))
   | Source.Bop_xor => existT _ _ (existT _ _ (existT _ _ Target.Bop_xor))
@@ -106,9 +107,10 @@ Definition translate_binop (op: Source.binop): { tin1 & { tin2 & { tout & Target
   | Source.Bop_lt => existT _ _ (existT _ _ (existT _ _ Target.Bop_lt))
   | Source.Bop_ge => existT _ _ (existT _ _ (existT _ _ Target.Bop_ge))
   | Source.Bop_gt => existT _ _ (existT _ _ (existT _ _ Target.Bop_gt))
-  | Source.Bop_arrow => existT _ _ (existT _ _ (existT _ _ Target.Bop_arrow))
-  | Source.Bop_fby => existT _ _ (existT _ _ (existT _ _ Target.Bop_arrow))
+  | Source.Bop_arrow => existT _ _ (existT _ _ (existT _ _ (@Target.Bop_arrow ty)))
+  | Source.Bop_fby => existT _ _ (existT _ _ (existT _ _ (@Target.Bop_arrow ty)))
 end.
+
 Definition typecheck_exp {P : forall ty, Target.exp ty -> Prop} (loc: Result.location) (e: { ty & sig (P ty) }) (t: type):
     Result.t type (sig (P t)) := match e, t with
   | existT _ TVoid (exist _ e H), TVoid => Result.Ok (exist _ e H)
@@ -136,6 +138,7 @@ Proof.
     exact eqty.
   - refine (Result.bind (check_exp temp e) _).
     intros e'.
+    destru
     destruct (translate_unop op) as [ tin [ tout top ]].
     refine (Result.bind (typecheck_exp l e' tin) _).
     intros [ e'' He ].
